code/bignum/Hacl.Bignum.AlmostMontExponentiation.fst
@@ -22,23 +22,28 @@ module BM = Hacl.Bignum.Montgomery
 module AM = Hacl.Bignum.AlmostMontgomery
 
 module LE = Lib.Exponentiation
-module SE = Spec.Exponentiation
 module BE = Hacl.Impl.Exponentiation
 module E = Hacl.Spec.Exponentiation.Lemmas
 module A = Hacl.Spec.AlmostMontgomery.Lemmas
+module M = Hacl.Spec.Montgomery.Lemmas
 module ME = Hacl.Spec.Bignum.MontExponentiation
 
 module S = Hacl.Spec.Bignum.AlmostMontExponentiation
 
 #reset-options "--z3rlimit 50 --fuel 0 --ifuel 0"
 
+
+inline_for_extraction noextract
+let a_spec (#t:limb_t) (#len:SN.bn_len t) (n:BD.lbignum t len{0 < BD.bn_v n}) =
+  Lib.NatMod.nat_mod (BD.bn_v n)
+
 inline_for_extraction noextract
 let linv (#t:limb_t) (#len:SN.bn_len t) (n:BD.lbignum t len) (a:BD.lbignum t len) : Type0 =
   BD.bn_v a < pow2 (bits t * len)
 
 inline_for_extraction noextract
-let refl (#t:limb_t) (#len:SN.bn_len t) (n:BD.lbignum t len{0 < BD.bn_v n}) (a:BD.lbignum t len{linv n a}) : BD.lbignum t len =
-  a
+let refl (#t:limb_t) (#len:SN.bn_len t) (n:BD.lbignum t len{0 < BD.bn_v n}) (a:BD.lbignum t len{linv n a}) : a_spec n =
+  BD.bn_v a % BD.bn_v n
 
 inline_for_extraction noextract
 let linv_ctx (#t:limb_t) (#len:SN.bn_len t) (n:BD.lbignum t len) (ctx:BD.lbignum t (len + len)) : Type0 =
@@ -49,15 +54,15 @@ let linv_ctx (#t:limb_t) (#len:SN.bn_len t) (n:BD.lbignum t len) (ctx:BD.lbignum
 
 
 inline_for_extraction noextract
-let mk_to_bn_mont_ll_concr_ops
+let mk_to_nat_mont_ll_comm_monoid
   (t:limb_t)
   (len:BN.meta_len t)
   (n:BD.lbignum t (v len))
   (mu:limb t{SM.bn_mont_pre n mu})
-  : BE.to_concrete_ops t len (len +! len) =
+  : BE.to_comm_monoid t len (len +! len) =
 {
-  BE.t_spec = BD.lbignum t (v len);
-  BE.concr_ops = S.mk_bn_almost_mont_concrete_ops n mu;
+  BE.a_spec = a_spec n;
+  BE.comm_monoid = E.mk_nat_mont_ll_comm_monoid (bits t) (v len) (BD.bn_v n) (v mu);
   BE.linv_ctx = linv_ctx n;
   BE.linv = linv n;
   BE.refl = refl n;
@@ -71,17 +76,24 @@ val bn_almost_mont_one:
   -> n:Ghost.erased (BD.lbignum t (v k.AM.bn.BN.len))
   -> mu:limb t{SM.bn_mont_pre n mu} ->
   BE.lone_st t k.AM.bn.BN.len (k.AM.bn.BN.len +! k.AM.bn.BN.len)
-    (mk_to_bn_mont_ll_concr_ops t k.AM.bn.BN.len n mu)
+    (mk_to_nat_mont_ll_comm_monoid t k.AM.bn.BN.len n mu)
 
 let bn_almost_mont_one #t k n mu ctx oneM =
   [@inline_let] let len = k.AM.bn.BN.len in
+  let k1 = Ghost.hide (E.mk_nat_mont_ll_comm_monoid (bits t) (v len) (BD.bn_v n) (v mu)) in
   let ctx_n = sub ctx 0ul len in
   let ctx_r2 = sub ctx len len in
   let h0 = ST.get () in
-  SM.bn_mont_one_lemma n mu (as_seq h0 ctx_r2);
   BM.bn_mont_one len k.AM.from ctx_n mu ctx_r2 oneM;
-  SM.bn_precomp_r2_mod_n_lemma 0 n;
-  BD.bn_eval_inj (v len) (SM.bn_precomp_r2_mod_n 0 n) (as_seq h0 ctx_r2)
+  let h1 = ST.get () in
+  SM.bn_mont_one_lemma n mu (as_seq h0 ctx_r2);
+  assert (BD.bn_v (as_seq h1 oneM) == M.mont_one (bits t) (v len) (BD.bn_v n) (v mu));
+  assert (BD.bn_v (as_seq h1 oneM) < BD.bn_v n);
+  BD.bn_eval_bound n (v len);
+  assert (linv n (as_seq h1 oneM));
+  Math.Lemmas.small_mod (BD.bn_v (as_seq h1 oneM)) (BD.bn_v n);
+  assert (BD.bn_v (as_seq h1 oneM) % BD.bn_v n ==
+    E.mont_one_ll (bits t) (v len) (BD.bn_v n) (v mu))
 
 
 inline_for_extraction noextract
@@ -91,7 +103,7 @@ val bn_almost_mont_mul:
   -> n:Ghost.erased (BD.lbignum t (v k.AM.bn.BN.len))
   -> mu:limb t{SM.bn_mont_pre n mu} ->
   BE.lmul_st t k.AM.bn.BN.len (k.AM.bn.BN.len +! k.AM.bn.BN.len)
-    (mk_to_bn_mont_ll_concr_ops t k.AM.bn.BN.len n mu)
+    (mk_to_nat_mont_ll_comm_monoid t k.AM.bn.BN.len n mu)
 
 let bn_almost_mont_mul #t k n mu ctx aM bM resM =
   let h0 = ST.get () in
@@ -108,7 +120,7 @@ val bn_almost_mont_sqr:
   -> n:Ghost.erased (BD.lbignum t (v k.AM.bn.BN.len))
   -> mu:limb t{SM.bn_mont_pre n mu} ->
   BE.lsqr_st t k.AM.bn.BN.len (k.AM.bn.BN.len +! k.AM.bn.BN.len)
-    (mk_to_bn_mont_ll_concr_ops t k.AM.bn.BN.len n mu)
+    (mk_to_nat_mont_ll_comm_monoid t k.AM.bn.BN.len n mu)
 
 let bn_almost_mont_sqr #t k n mu ctx aM resM =
   let h0 = ST.get () in
@@ -127,7 +139,7 @@ let mk_bn_almost_mont_concrete_ops
   (mu:limb t{SM.bn_mont_pre n mu}) :
   BE.concrete_ops t k.AM.bn.BN.len (k.AM.bn.BN.len +! k.AM.bn.BN.len) =
 {
-  BE.to = mk_to_bn_mont_ll_concr_ops t k.AM.bn.BN.len n mu;
+  BE.to = mk_to_nat_mont_ll_comm_monoid t k.AM.bn.BN.len n mu;
   BE.lone = bn_almost_mont_one k n mu;
   BE.lmul = bn_almost_mont_mul k n mu;
   BE.lsqr = bn_almost_mont_sqr k n mu;
@@ -216,7 +228,6 @@ let bn_exp_almost_mont_bm_vartime #t k n mu r2 aM bBits b resM =
 
   BD.bn_eval_bound (as_seq h0 aM) (v len);
   BE.lexp_rl_vartime len (len +! len) (mk_bn_almost_mont_concrete_ops t k (as_seq h0 n) mu) ctx aM bLen bBits b resM;
-  SE.exp_rl_lemma (S.mk_bn_almost_mont_concrete_ops (as_seq h0 n) mu) (as_seq h0 aM) (v bBits) (bn_v h0 b);
   LE.exp_rl_lemma k1 (bn_v h0 aM % bn_v h0 n) (v bBits) (bn_v h0 b);
   E.pow_nat_mont_ll_mod_base (bits t) (v len) (bn_v h0 n) (v mu) (bn_v h0 aM) (bn_v h0 b);
   pop_frame ()
@@ -235,7 +246,6 @@ let bn_exp_almost_mont_bm_consttime #t k n mu r2 aM bBits b resM =
   mk_ctx #t len n r2 ctx;
 
   BE.lexp_mont_ladder_swap_consttime len (len +! len) (mk_bn_almost_mont_concrete_ops t k (as_seq h0 n) mu) ctx aM bLen bBits b resM;
-  SE.exp_mont_ladder_swap_lemma (S.mk_bn_almost_mont_concrete_ops (as_seq h0 n) mu) (as_seq h0 aM) (v bBits) (bn_v h0 b);
   LE.exp_mont_ladder_swap_lemma k1 (bn_v h0 aM % bn_v h0 n) (v bBits) (bn_v h0 b);
   LE.exp_mont_ladder_lemma k1 (bn_v h0 aM % bn_v h0 n) (v bBits) (bn_v h0 b);
   E.pow_nat_mont_ll_mod_base (bits t) (v len) (bn_v h0 n) (v mu) (bn_v h0 aM) (bn_v h0 b);
@@ -260,7 +270,6 @@ let bn_exp_almost_mont_fw_vartime #t k l n mu r2 aM bBits b resM =
   mk_ctx #t len n r2 ctx;
 
   BE.lexp_fw_vartime len (len +! len) (mk_bn_almost_mont_concrete_ops t k (as_seq h0 n) mu) l ctx aM bLen bBits b resM;
-  SE.exp_fw_lemma (S.mk_bn_almost_mont_concrete_ops (as_seq h0 n) mu) (as_seq h0 aM) (v bBits) (bn_v h0 b) (v l);
   LE.exp_fw_lemma k1 (bn_v h0 aM % bn_v h0 n) (v bBits) (bn_v h0 b) (v l);
   E.pow_nat_mont_ll_mod_base (bits t) (v len) (bn_v h0 n) (v mu) (bn_v h0 aM) (bn_v h0 b);
   pop_frame ()
@@ -284,7 +293,6 @@ let bn_exp_almost_mont_fw_consttime #t k l n mu r2 aM bBits b resM =
   mk_ctx #t len n r2 ctx;
 
   BE.lexp_fw_consttime len (len +! len) (mk_bn_almost_mont_concrete_ops t k (as_seq h0 n) mu) l ctx aM bLen bBits b resM;
-  SE.exp_fw_lemma (S.mk_bn_almost_mont_concrete_ops (as_seq h0 n) mu) (as_seq h0 aM) (v bBits) (bn_v h0 b) (v l);
   LE.exp_fw_lemma k1 (bn_v h0 aM % bn_v h0 n) (v bBits) (bn_v h0 b) (v l);
   E.pow_nat_mont_ll_mod_base (bits t) (v len) (bn_v h0 n) (v mu) (bn_v h0 aM) (bn_v h0 b);
   pop_frame ()
