code/bignum/Hacl.Impl.Exponentiation.Definitions.fst
@@ -9,7 +9,7 @@ open Lib.Buffer
 
 module ST = FStar.HyperStack.ST
 module LSeq = Lib.Sequence
-module SE = Spec.Exponentiation
+module S = Lib.Exponentiation
 
 #reset-options "--z3rlimit 50 --fuel 0 --ifuel 0"
 
@@ -17,12 +17,12 @@ inline_for_extraction noextract
 let inttype_a = t:inttype{t = U32 \/ t = U64}
 
 inline_for_extraction noextract
-class to_concrete_ops (a_t:inttype_a) (len:size_t{v len > 0}) (ctx_len:size_t) = {
-  t_spec: Type0;
-  concr_ops: SE.concrete_ops t_spec;
+class to_comm_monoid (a_t:inttype_a) (len:size_t{v len > 0}) (ctx_len:size_t) = {
+  a_spec: Type0;
+  comm_monoid: S.comm_monoid a_spec;
   linv_ctx: x:LSeq.lseq (uint_t a_t SEC) (v ctx_len) -> Type0;
   linv: x:LSeq.lseq (uint_t a_t SEC) (v len) -> Type0;
-  refl: x:LSeq.lseq (uint_t a_t SEC) (v len){linv x} -> GTot t_spec;
+  refl: x:LSeq.lseq (uint_t a_t SEC) (v len){linv x} -> GTot a_spec;
 }
 
 
@@ -31,7 +31,7 @@ let lone_st
   (a_t:inttype_a)
   (len:size_t{v len > 0})
   (ctx_len:size_t)
-  (to:to_concrete_ops a_t len ctx_len) =
+  (to:to_comm_monoid a_t len ctx_len) =
     ctx:lbuffer (uint_t a_t SEC) ctx_len
   -> x:lbuffer (uint_t a_t SEC) len ->
   Stack unit
@@ -40,7 +40,7 @@ let lone_st
     to.linv_ctx (as_seq h ctx))
   (ensures  fun h0 _ h1 -> modifies (loc x) h0 h1 /\
     to.linv (as_seq h1 x) /\
-    to.refl (as_seq h1 x) == to.concr_ops.SE.one ())
+    to.refl (as_seq h1 x) == to.comm_monoid.S.one)
 
 
 inline_for_extraction noextract
@@ -48,7 +48,7 @@ let lmul_st
   (a_t:inttype_a)
   (len:size_t{v len > 0})
   (ctx_len:size_t)
-  (to:to_concrete_ops a_t len ctx_len) =
+  (to:to_comm_monoid a_t len ctx_len) =
     ctx:lbuffer (uint_t a_t SEC) ctx_len
   -> x:lbuffer (uint_t a_t SEC) len
   -> y:lbuffer (uint_t a_t SEC) len
@@ -60,7 +60,7 @@ let lmul_st
     disjoint ctx x /\ disjoint ctx y /\ disjoint ctx xy /\
     to.linv (as_seq h x) /\ to.linv (as_seq h y) /\ to.linv_ctx (as_seq h ctx))
   (ensures fun h0 _ h1 -> modifies (loc xy) h0 h1 /\ to.linv (as_seq h1 xy) /\
-    to.refl (as_seq h1 xy) == to.concr_ops.SE.mul (to.refl (as_seq h0 x)) (to.refl (as_seq h0 y)))
+    to.refl (as_seq h1 xy) == to.comm_monoid.S.mul (to.refl (as_seq h0 x)) (to.refl (as_seq h0 y)))
 
 
 inline_for_extraction noextract
@@ -68,7 +68,7 @@ let lsqr_st
   (a_t:inttype_a)
   (len:size_t{v len > 0})
   (ctx_len:size_t)
-  (to:to_concrete_ops a_t len ctx_len) =
+  (to:to_comm_monoid a_t len ctx_len) =
     ctx:lbuffer (uint_t a_t SEC) ctx_len
   -> x:lbuffer (uint_t a_t SEC) len
   -> xx:lbuffer (uint_t a_t SEC) len ->
@@ -78,12 +78,12 @@ let lsqr_st
     disjoint x ctx /\ disjoint xx ctx /\ eq_or_disjoint x xx /\
     to.linv (as_seq h x) /\ to.linv_ctx (as_seq h ctx))
   (ensures fun h0 _ h1 -> modifies (loc xx) h0 h1 /\ to.linv (as_seq h1 xx) /\
-    to.refl (as_seq h1 xx) == to.concr_ops.SE.sqr (refl (as_seq h0 x)))
+    to.refl (as_seq h1 xx) == to.comm_monoid.S.mul (refl (as_seq h0 x)) (refl (as_seq h0 x)))
 
 
 inline_for_extraction noextract
 class concrete_ops (a_t:inttype_a) (len:size_t{v len > 0}) (ctx_len:size_t) = {
-  to: Ghost.erased (to_concrete_ops a_t len ctx_len);
+  to: Ghost.erased (to_comm_monoid a_t len ctx_len);
   lone: lone_st a_t len ctx_len to;
   lmul: lmul_st a_t len ctx_len to;
   lsqr: lsqr_st a_t len ctx_len to;
