code/k256/Hacl.Impl.K256.PointMul.fst
@@ -10,10 +10,12 @@ open Lib.Buffer
 module ST = FStar.HyperStack.ST
 module LSeq = Lib.Sequence
 
+module SE = Spec.Exponentiation
 module BE = Hacl.Impl.Exponentiation
 module ME = Hacl.Impl.MultiExponentiation
 
 module S = Spec.K256
+module SL = Spec.K256.Lemmas
 
 open Hacl.K256.Field
 open Hacl.K256.Scalar
@@ -27,13 +29,13 @@ unfold
 let linv_ctx (a:LSeq.lseq uint64 0) : Type0 = True
 
 unfold
-let refl (p:LSeq.lseq uint64 15{point_inv_lseq p}) : GTot S.proj_point =
-  point_eval_lseq p
+let refl (p:LSeq.lseq uint64 15{point_inv_lseq p}) : GTot S.aff_point =
+  S.to_aff_point (point_eval_lseq p)
 
 inline_for_extraction noextract
-let mk_to_k256_concrete_ops : BE.to_concrete_ops U64 15ul 0ul = {
-  BE.t_spec = S.proj_point;
-  BE.concr_ops = S.mk_k256_concrete_ops;
+let mk_to_k256_comm_monoid : BE.to_comm_monoid U64 15ul 0ul = {
+  BE.a_spec = S.aff_point;
+  BE.comm_monoid = S.mk_k256_comm_monoid;
   BE.linv_ctx = linv_ctx;
   BE.linv = point_inv_lseq;
   BE.refl = refl;
@@ -41,23 +43,28 @@ let mk_to_k256_concrete_ops : BE.to_concrete_ops U64 15ul 0ul = {
 
 
 inline_for_extraction noextract
-val point_add : BE.lmul_st U64 15ul 0ul mk_to_k256_concrete_ops
+val point_add : BE.lmul_st U64 15ul 0ul mk_to_k256_comm_monoid
 let point_add ctx x y xy =
+  let h0 = ST.get () in
+  SL.to_aff_point_add_lemma (point_eval h0 x) (point_eval h0 y);
   Hacl.Impl.K256.PointAdd.point_add xy x y
 
 
 inline_for_extraction noextract
-val point_double : BE.lsqr_st U64 15ul 0ul mk_to_k256_concrete_ops
+val point_double : BE.lsqr_st U64 15ul 0ul mk_to_k256_comm_monoid
 let point_double ctx x xx =
+  let h0 = ST.get () in
+  SL.to_aff_point_double_lemma (point_eval h0 x);
   Hacl.Impl.K256.PointDouble.point_double xx x
 
 
 val make_point_at_inf: p:point -> Stack unit
   (requires fun h -> live h p)
   (ensures  fun h0 _ h1 -> modifies (loc p) h0 h1 /\
-    point_inv h1 p /\ point_eval h1 p == S.point_at_inf)
+    point_inv h1 p /\ S.to_aff_point (point_eval h1 p) == S.aff_point_at_inf)
 
 let make_point_at_inf p =
+  SL.to_aff_point_at_infinity_lemma ();
   let px, py, pz = getx p, gety p, getz p in
   set_zero px;
   set_one py;
@@ -65,13 +72,13 @@ let make_point_at_inf p =
 
 
 inline_for_extraction noextract
-val point_zero : BE.lone_st U64 15ul 0ul mk_to_k256_concrete_ops
+val point_zero : BE.lone_st U64 15ul 0ul mk_to_k256_comm_monoid
 let point_zero ctx one = make_point_at_inf one
 
 
 inline_for_extraction noextract
 let mk_k256_concrete_ops : BE.concrete_ops U64 15ul 0ul = {
-  BE.to = mk_to_k256_concrete_ops;
+  BE.to = mk_to_k256_comm_monoid;
   BE.lone = point_zero;
   BE.lmul = point_add;
   BE.lsqr = point_double;
@@ -83,8 +90,7 @@ inline_for_extraction noextract
 val make_g: g:point -> Stack unit
   (requires fun h -> live h g)
   (ensures  fun h0 _ h1 -> modifies (loc g) h0 h1 /\
-    point_inv h1 g /\
-    point_eval h1 g == S.g)
+    point_inv h1 g /\ point_eval h1 g == S.g)
 
 let make_g g =
   let gx, gy, gz = getx g, gety g, getz g in
@@ -123,9 +129,12 @@ val point_mul: out:point -> scalar:qelem -> q:point -> Stack unit
     point_inv h q /\ qas_nat h scalar < S.q)
   (ensures  fun h0 _ h1 -> modifies (loc out) h0 h1 /\
     point_inv h1 out /\
-    point_eval h1 out == S.point_mul (qas_nat h0 scalar) (point_eval h0 q))
+    S.to_aff_point (point_eval h1 out) ==
+    S.to_aff_point (S.point_mul (qas_nat h0 scalar) (point_eval h0 q)))
 
 let point_mul out scalar q =
+  let h0 = ST.get () in
+  SE.exp_fw_lemma S.mk_k256_concrete_ops (point_eval h0 q) 256 (qas_nat h0 scalar) 4;
   BE.lexp_fw_consttime 15ul 0ul mk_k256_concrete_ops 4ul (null uint64) q 4ul 256ul scalar out
 
 
@@ -139,13 +148,17 @@ val point_mul_double_vartime:
     qas_nat h scalar1 < S.q /\ qas_nat h scalar2 < S.q)
   (ensures fun h0 _ h1 -> modifies (loc out) h0 h1 /\
     point_inv h1 out /\
-    point_eval h1 out ==
-    S.point_mul_double
+    S.to_aff_point (point_eval h1 out) ==
+    S.to_aff_point (S.point_mul_double
       (qas_nat h0 scalar1) (point_eval h0 q1)
-      (qas_nat h0 scalar2) (point_eval h0 q2))
+      (qas_nat h0 scalar2) (point_eval h0 q2)))
 
 [@CInline]
 let point_mul_double_vartime out scalar1 q1 scalar2 q2 =
+  let h0 = ST.get () in
+  SE.exp_double_fw_lemma S.mk_k256_concrete_ops
+    (point_eval h0 q1) 256 (qas_nat h0 scalar1)
+    (point_eval h0 q2) (qas_nat h0 scalar2) 4;
   ME.lexp_double_fw_vartime 15ul 0ul mk_k256_concrete_ops 4ul (null uint64) q1 4ul 256ul scalar1 q2 scalar2 out
 
 
@@ -155,7 +168,8 @@ val point_mul_g: out:point -> scalar:qelem -> Stack unit
     qas_nat h scalar < S.q)
   (ensures  fun h0 _ h1 -> modifies (loc out) h0 h1 /\
     point_inv h1 out /\
-    point_eval h1 out == S.point_mul_g (qas_nat h0 scalar))
+    S.to_aff_point (point_eval h1 out) ==
+    S.to_aff_point (S.point_mul_g (qas_nat h0 scalar)))
 
 [@CInline]
 let point_mul_g out scalar =
@@ -174,9 +188,9 @@ val point_mul_g_double_vartime: out:point -> scalar1:qelem -> scalar2:qelem -> q
     point_inv h q2 /\ qas_nat h scalar1 < S.q /\ qas_nat h scalar2 < S.q)
   (ensures fun h0 _ h1 -> modifies (loc out) h0 h1 /\
     point_inv h1 out /\
-    point_eval h1 out ==
-    S.point_mul_double_g
-      (qas_nat h0 scalar1) (qas_nat h0 scalar2) (point_eval h0 q2))
+    S.to_aff_point (point_eval h1 out) ==
+    S.to_aff_point (S.point_mul_double_g
+      (qas_nat h0 scalar1) (qas_nat h0 scalar2) (point_eval h0 q2)))
 
 [@CInline]
 let point_mul_g_double_vartime out scalar1 scalar2 q2 =
