code/k256/Hacl.Impl.K256.Verify.fst
@@ -160,6 +160,36 @@ let ecdsa_verify_avoid_finv p r =
 
 
 inline_for_extraction noextract
+let spec_ecdsa_verify_qelem_aff (pk_x pk_y:S.felem) (z r s:S.qelem) : S.aff_point =
+  let pk_aff  = (pk_x, pk_y) in
+  let pk_proj = S.to_proj_point pk_aff in
+  let g_aff   = (S.g_x, S.g_y) in
+  let sinv = S.qinv s in
+  let u1 = S.qmul z sinv in
+  let u2 = S.qmul r sinv in
+  S.aff_point_add (S.aff_point_mul u1 g_aff) (S.aff_point_mul u2 pk_aff)
+
+
+val lemma_spec_ecdsa_verify_qelem_aff (pk_x pk_y:S.felem) (z r s:S.qelem) : Lemma
+  (let sinv = S.qinv s in let u1 = S.qmul z sinv in let u2 = S.qmul r sinv in
+  S.to_aff_point (S.point_mul_double_g u1 u2 (S.to_proj_point (pk_x, pk_y))) ==
+    spec_ecdsa_verify_qelem_aff pk_x pk_y z r s)
+
+let lemma_spec_ecdsa_verify_qelem_aff pk_x pk_y z r s =
+  let pk_aff  = (pk_x, pk_y) in
+  let pk_proj = S.to_proj_point pk_aff in
+  let g_aff   = (S.g_x, S.g_y) in
+  let sinv = S.qinv s in
+  let u1 = S.qmul z sinv in
+  let u2 = S.qmul r sinv in
+  Hacl.Spec.K256.ECSM.Lemmas.lemma_proj_aff_id g_aff;
+  Hacl.Spec.K256.ECSM.Lemmas.lemma_proj_aff_id pk_aff;
+  SE.exp_double_fw_lemma S.mk_k256_concrete_ops S.g 256 u1 pk_proj u2 4;
+  LE.exp_double_fw_lemma S.mk_k256_comm_monoid
+    (S.to_aff_point S.g) 256 u1 (S.to_aff_point pk_proj) u2 4
+
+
+inline_for_extraction noextract
 val ecdsa_verify_qelem_aff (pk_x pk_y:felem) (z r s:QA.qelem) : Stack bool
   (requires fun h ->
     live h pk_x /\ live h pk_y /\ live h z /\ live h r /\ live h s /\
@@ -177,20 +207,10 @@ val ecdsa_verify_qelem_aff (pk_x pk_y:felem) (z r s:QA.qelem) : Stack bool
 
 let ecdsa_verify_qelem_aff pk_x pk_y z r s =
   let h0 = ST.get () in
-  let pk_aff = Ghost.hide ((feval h0 pk_x, feval h0 pk_y)) in
-  let pk_proj = Ghost.hide (S.to_proj_point (feval h0 pk_x, feval h0 pk_y)) in
-  let g_aff = Ghost.hide (S.g_x, S.g_y) in
-  Hacl.Spec.K256.ECSM.Lemmas.lemma_proj_aff_id g_aff;
-  Hacl.Spec.K256.ECSM.Lemmas.lemma_proj_aff_id pk_aff;
-  let sinv = Ghost.hide (S.qinv (QA.qas_nat h0 s)) in
-  let u1 = Ghost.hide (S.qmul (QA.qas_nat h0 z) sinv) in
-  let u2 = Ghost.hide (S.qmul (QA.qas_nat h0 r) sinv) in
-  SE.exp_double_fw_lemma S.mk_k256_concrete_ops S.g 256 u1 pk_proj u2 4;
-  LE.exp_double_fw_lemma S.mk_k256_comm_monoid
-    (S.to_aff_point S.g) 256 u1 (S.to_aff_point pk_proj) u2 4;
-  assert (S.to_aff_point (S.point_mul_double_g u1 u2 pk_proj) ==
-    S.aff_point_add (S.aff_point_mul u1 (S.g_x, S.g_y)) (S.aff_point_mul u2 pk_aff));
-
+  Hacl.Spec.K256.ECSM.Lemmas.lemma_proj_aff_id (S.g_x, S.g_y);
+  Hacl.Spec.K256.ECSM.Lemmas.lemma_proj_aff_id (feval h0 pk_x, feval h0 pk_y);
+  lemma_spec_ecdsa_verify_qelem_aff (feval h0 pk_x) (feval h0 pk_y)
+    (QA.qas_nat h0 z) (QA.qas_nat h0 r) (QA.qas_nat h0 s);
   push_frame ();
   let p = create_point () in
   let res = create_point () in
